Logic/Predicate/FirstOrder/Computability/Calculus.lean
@@ -1,0 +1,227 @@
+import Logic.Predicate.FirstOrder.Computability.Term
+import Logic.Predicate.FirstOrder.Computability.Formula
+import Logic.Predicate.FirstOrder.Basic.Calculus
+import Logic.Predicate.FirstOrder.Hauptsatz
+
+namespace LO
+
+namespace FirstOrder
+
+open Encodable Primrec
+variable {L : Language.{u}} [∀ k, DecidableEq (L.func k)] [∀ k, DecidableEq (L.rel k)]
+variable [(k : ℕ) → Primcodable (L.func k)] [(k : ℕ) → Primcodable (L.rel k)]
+  [UniformlyPrimcodable L.func] [UniformlyPrimcodable L.rel] [Primcodable μ]
+
+namespace Derivation
+
+open DerivationCR
+
+inductive Code (L : Language.{u})
+  | axL : {k : ℕ} → (r : L.rel k) → (v : Fin k → SyntacticTerm L) → Code L
+  | verum : Code L
+  | and : SyntacticFormula L → SyntacticFormula L → Code L
+  | or : SyntacticFormula L → SyntacticFormula L → Code L
+  | all : SyntacticSubFormula L 1 → Code L
+  | ex : SyntacticSubFormula L 1 → SyntacticTerm L → Code L
+  | wk : List (SyntacticFormula L) → Code L
+
+def Code.equiv (L : Language.{u}) :
+    Code L ≃
+    ((k : ℕ) × (L.rel k) × (Fin k → SyntacticTerm L)) ⊕
+    Unit ⊕
+    (SyntacticFormula L × SyntacticFormula L) ⊕
+    (SyntacticFormula L × SyntacticFormula L) ⊕
+    (SyntacticSubFormula L 1) ⊕
+    (SyntacticSubFormula L 1 × SyntacticTerm L) ⊕
+    List (SyntacticFormula L) where
+  toFun := fun c =>
+    match c with
+    | (Code.axL r v) => Sum.inl ⟨_, r, v⟩
+    | Code.verum     => Sum.inr $ Sum.inl ()
+    | (Code.and p q) => Sum.inr $ Sum.inr $ Sum.inl (p, q)
+    | (Code.or p q)  => Sum.inr $ Sum.inr $ Sum.inr $ Sum.inl (p, q)
+    | (Code.all p)   => Sum.inr $ Sum.inr $ Sum.inr $ Sum.inr $ Sum.inl p
+    | (Code.ex p t)  => Sum.inr $ Sum.inr $ Sum.inr $ Sum.inr $ Sum.inr $ Sum.inl (p, t)
+    | (Code.wk Δ)    => Sum.inr $ Sum.inr $ Sum.inr $ Sum.inr $ Sum.inr $ Sum.inr Δ
+  invFun := fun x =>
+    match x with
+    | (Sum.inl ⟨_, r, v⟩)                                                => Code.axL r v
+    | (Sum.inr $ Sum.inl ())                                             => Code.verum
+    | (Sum.inr $ Sum.inr $ Sum.inl (p, q))                               => Code.and p q
+    | (Sum.inr $ Sum.inr $ Sum.inr $ Sum.inl (p, q))                     => Code.or p q
+    | (Sum.inr $ Sum.inr $ Sum.inr $ Sum.inr $ Sum.inl p)                => Code.all p
+    | (Sum.inr $ Sum.inr $ Sum.inr $ Sum.inr $ Sum.inr $ Sum.inl (p, t)) => Code.ex p t
+    | (Sum.inr $ Sum.inr $ Sum.inr $ Sum.inr $ Sum.inr $ Sum.inr Δ)      => Code.wk Δ
+  left_inv := fun c => by cases c <;> simp
+  right_inv := fun x => by
+    rcases x with (⟨_, _, _⟩ | ⟨⟩ | ⟨_, _⟩ | ⟨_, _⟩ | _ | ⟨_, _⟩ | _) <;> simp
+
+instance : Primcodable (Code L) := Primcodable.ofEquiv _ (Code.equiv L)
+
+abbrev ProofList (L : Language.{u}) := List (Code L × List (SyntacticFormula L))
+
+namespace ProofList
+
+def sequents : ProofList L → List (List (SyntacticFormula L)) := List.map Prod.snd
+
+def isProper : ProofList L → Bool
+  | []                     => true
+  | (Code.axL r v, Γ) :: l => isProper l && SubFormula.rel r v ∈ Γ && SubFormula.nrel r v ∈ Γ
+  | (Code.verum,   Γ) :: l => isProper l && ⊤ ∈ Γ
+  | (Code.and p q, Γ) :: l => isProper l && p ⋏ q ∈ Γ && p :: Γ ∈ sequents l && q :: Γ ∈ sequents l
+  | (Code.or p q,  Γ) :: l => isProper l && p ⋎ q ∈ Γ && p :: q :: Γ ∈ sequents l
+  | (Code.all p,   Γ) :: l => isProper l && ∀' p ∈ Γ && Rew.freel p :: Γ.map Rew.shiftl ∈ sequents l
+  | (Code.ex p t,  Γ) :: l => isProper l && ∃' p ∈ Γ && Rew.substsl ![t] p :: Γ ∈ sequents l
+  | (Code.wk Δ,    Γ) :: l => isProper l && Δ ⊆ Γ && Δ ∈ sequents l
+
+@[simp] lemma sequents_append {l₁ l₂ : ProofList L} : sequents (l₁ ++ l₂) = sequents l₁ ++ sequents l₂ := by simp[sequents]
+
+lemma isProper_append {l₁ l₂ : ProofList L} (h₁ : isProper l₁) (h₂ : isProper l₂) : isProper (l₁ ++ l₂) := by
+  induction' l₁ with c l₁ ih
+  · simpa
+  · simp
+    rcases c with ⟨⟨⟩, Γ⟩ <;> simp[isProper] at h₁ ⊢
+    case axL k r v => { exact ⟨⟨ih h₁.1.1, h₁.1.2⟩, h₁.2⟩ }
+    case verum => { exact ⟨ih h₁.1, h₁.2⟩ }
+    case and p q => { exact ⟨⟨⟨ih h₁.1.1.1, h₁.1.1.2⟩, Or.inl h₁.1.2⟩, Or.inl h₁.2⟩ }
+    case or p q => { exact ⟨⟨ih h₁.1.1, h₁.1.2⟩, Or.inl h₁.2⟩ }
+    case all => { exact ⟨⟨ih h₁.1.1, h₁.1.2⟩, Or.inl h₁.2⟩ }
+    case ex => { exact ⟨⟨ih h₁.1.1, h₁.1.2⟩, Or.inl h₁.2⟩ }
+    case wk => { exact ⟨⟨ih h₁.1.1, h₁.1.2⟩, Or.inl h₁.2⟩ }
+
+def head : List (Code L × List (SyntacticFormula L)) → List (SyntacticFormula L)
+  | []          => [⊤]
+  | ⟨_, Γ⟩ :: _ => Γ
+
+lemma derivation_of_isProper : (l : ProofList L) → isProper l → ∀ Γ ∈ sequents l, Nonempty (⊢ᵀ Γ.toFinset)
+  | [],                     _, Δ, hΔ => by simp[sequents] at hΔ
+  | (Code.axL r v, Γ) :: l, H, Δ, hΔ => by
+    simp[isProper] at H; rcases H with ⟨⟨ih, h₁⟩, h₂⟩
+    simp[sequents] at hΔ; rcases hΔ with (rfl | hΔ)
+    · exact ⟨axL _ r v (by simpa using h₁) (by simpa using h₂)⟩
+    · exact derivation_of_isProper l ih Δ (by simpa[sequents] using hΔ)
+  | (Code.verum,   Γ) :: l, H, Δ, hΔ => by
+    simp[isProper] at H; rcases H with ⟨ih, h⟩
+    simp[sequents] at hΔ; rcases hΔ with (rfl | hΔ)
+    · exact ⟨verum _ (by simp[h])⟩
+    · exact derivation_of_isProper l ih _ (by simpa[sequents] using hΔ)
+  | (Code.and p q, Γ) :: l, H, Δ, hΔ => by
+    simp[isProper] at H; rcases H with ⟨⟨⟨hl, H⟩, hp⟩, hq⟩
+    simp[sequents] at hΔ; rcases hΔ with (rfl | hΔ)
+    · have : Nonempty (⊢ᵀ List.toFinset (p :: Δ)) := derivation_of_isProper l hl _ hp
+      rcases this with ⟨bp⟩
+      have : Nonempty (⊢ᵀ List.toFinset (q :: Δ)) := derivation_of_isProper l hl _ hq
+      rcases this with ⟨bq⟩
+      have : ⊢ᵀ insert (p ⋏ q) Δ.toFinset := and Δ.toFinset p q (by simpa using bp) (by simpa using bq)
+      exact ⟨this.cast (by simp[H])⟩
+    · exact derivation_of_isProper l hl _ (by simpa[sequents] using hΔ)
+  | (Code.or p q, Γ) :: l,  H, Δ, hΔ => by
+    simp[isProper] at H; rcases H with ⟨⟨hl, H⟩, hpq⟩
+    simp[sequents] at hΔ; rcases hΔ with (rfl | hΔ)
+    · rcases derivation_of_isProper l hl _ hpq with ⟨b⟩
+      have : ⊢ᵀ insert (p ⋎ q) Δ.toFinset := DerivationCR.or Δ.toFinset p q (by simpa using b)
+      exact ⟨this.cast (by simp[H])⟩
+    · exact derivation_of_isProper l hl _ (by simpa[sequents] using hΔ)
+  | (Code.all p, Γ) :: l,   H, Δ, hΔ => by
+    simp[isProper] at H; rcases H with ⟨⟨hl, H⟩, hp⟩
+    simp[sequents] at hΔ; rcases hΔ with (rfl | hΔ)
+    · rcases derivation_of_isProper l hl _ hp with ⟨b⟩
+      have : ⊢ᵀ insert (∀' p) Δ.toFinset :=
+        DerivationCR.all Δ.toFinset p (by simpa[shifts, List.toFinset_map, Finset.map_eq_image] using b)
+      exact ⟨this.cast (by simp[H])⟩
+    · exact derivation_of_isProper l hl _ (by simpa[sequents] using hΔ)
+  | (Code.ex p t, Γ) :: l,    H, Δ, hΔ => by
+    simp[isProper] at H; rcases H with ⟨⟨hl, H⟩, hp⟩
+    simp[sequents] at hΔ; rcases hΔ with (rfl | hΔ)
+    · rcases derivation_of_isProper l hl _ hp with ⟨b⟩
+      have : ⊢ᵀ insert (∃' p) Δ.toFinset := DerivationCR.ex Δ.toFinset t p (by simpa using b)
+      exact ⟨this.cast (by simp[H])⟩
+    · exact derivation_of_isProper l hl _ (by simpa[sequents] using hΔ)
+  | (Code.wk E,   Γ) :: l,    H, Δ, hΔ => by
+    simp[isProper] at H; rcases H with ⟨⟨hl, H⟩, h⟩
+    simp[sequents] at hΔ; rcases hΔ with (rfl | hΔ)
+    · rcases derivation_of_isProper l hl E h with ⟨b⟩
+      exact ⟨b.weakening (by intro x; simp; intro hx; exact H hx)⟩
+    · exact derivation_of_isProper l hl _ (by simpa[sequents] using hΔ)
+
+noncomputable def ofDerivation : {Γ : Sequent L} → ⊢ᵀ Γ → ProofList L
+  | _, DerivationCR.axL Γ r v _ _   => [(Code.axL r v, Γ.toList)]
+  | _, DerivationCR.verum Γ _       => [(Code.verum, Γ.toList)]
+  | _, DerivationCR.and Γ p q bp bq =>
+    (Code.and p q, (insert (p ⋏ q) Γ).toList) ::
+    (Code.wk (insert p Γ).toList, p :: (insert (p ⋏ q) Γ).toList) ::
+    (Code.wk (insert q Γ).toList, q :: (insert (p ⋏ q) Γ).toList) :: (ofDerivation bp ++ ofDerivation bq)
+  | _, DerivationCR.or Γ p q bpq    =>
+    (Code.or p q, (insert (p ⋎ q) Γ).toList) ::
+    (Code.wk (insert p $ insert q Γ).toList, p :: q :: (insert (p ⋎ q) Γ).toList) :: ofDerivation bpq
+  | _, DerivationCR.all Γ p b       =>
+    (Code.all p, (insert (∀' p) Γ).toList) ::
+    (Code.wk (insert (Rew.freel p) $ shifts Γ).toList, Rew.freel p :: (insert (∀' p) Γ).toList.map Rew.shiftl) :: ofDerivation b
+  | _, DerivationCR.ex Γ t p b      =>
+    (Code.ex p t, (insert (∃' p) Γ).toList) ::
+    (Code.wk (insert (Rew.substsl ![t] p) Γ).toList, Rew.substsl ![t] p :: (insert (∃' p) Γ).toList) :: ofDerivation b
+
+lemma mem_ofDerivation {Γ : Sequent L} (b : ⊢ᵀ Γ) : Γ.toList ∈ sequents (ofDerivation b) := by
+  cases b <;> simp[ofDerivation, sequents]
+  { contradiction }
+
+lemma iff_mem_sequents {l : ProofList L} : (∃ c, (c, Γ) ∈ l) ↔ Γ ∈ sequents l := by simp[sequents]
+
+@[simp] lemma sequents_cons {l : ProofList L} : sequents ((c, Γ) :: l) = Γ :: sequents l := by simp[sequents]
+
+lemma List.mem_cons_cons (l : List α) (a b : α) : l ⊆ a :: b :: l := by
+  intro x hx; simp; exact Or.inr (Or.inr $ hx)
+
+lemma Finset.mem_cons_cons [DecidableEq α] (s : Finset α) (a b : α) : s ⊆ insert a (insert b s) := by
+  intro x hx; simp; exact Or.inr (Or.inr $ hx)
+
+lemma Finset.toList_subset_toList {s₁ s₂ : Finset α} : s₁.toList ⊆ s₂.toList ↔ s₁ ⊆ s₂ := by
+  simp[List.subset_def]; rfl
+
+lemma isProper_ofDerivation : ∀ {Γ : Sequent L} (b : ⊢ᵀ Γ), isProper (ofDerivation b)
+  | _, DerivationCR.axL Γ r v h₁ h₂ => by simp[ofDerivation, isProper, h₁, h₂]
+  | _, DerivationCR.verum Γ h       => by simp[ofDerivation, isProper, h]
+  | _, DerivationCR.and Γ p q bp bq => by
+    simp[isProper, sequents_cons, List.mem_cons_cons, mem_ofDerivation]
+    exact ⟨⟨isProper_append (isProper_ofDerivation bp) (isProper_ofDerivation bq), by simp[List.subset_def]; intro x hx; exact Or.inr (Or.inr hx)⟩,
+      by simp[List.subset_def]; intro x hx; exact Or.inr (Or.inr hx)⟩
+  | _, DerivationCR.or Γ p q bpq    => by
+    simp[isProper, sequents_cons, List.mem_cons_cons, mem_ofDerivation]
+    exact ⟨isProper_ofDerivation bpq, by simp[List.subset_def]; intro x hx; simp[hx]⟩
+  | _, DerivationCR.all Γ p b       => by
+    simp[isProper, sequents_cons, List.mem_cons_cons, mem_ofDerivation]
+    exact ⟨isProper_ofDerivation b, by simp[List.subset_def, shifts_eq_image]; intro x hx; exact (Or.inr $ Or.inr $ ⟨x, hx, rfl⟩)⟩
+  | _, DerivationCR.ex Γ t p b      => by
+    simp[isProper, sequents_cons, List.mem_cons_cons, mem_ofDerivation]
+    exact ⟨isProper_ofDerivation b, by simp[List.subset_def]; intro x hx; simp[hx]⟩
+  
+lemma derivable_iff_isProper {Γ : Sequent L} : Nonempty (⊢ᵀ Γ) ↔ ∃ l, isProper l ∧ Γ.toList ∈ sequents l :=
+  ⟨by rintro ⟨b⟩; exact ⟨ofDerivation b, isProper_ofDerivation b, mem_ofDerivation b⟩,
+   by rintro ⟨l, hl⟩; rcases derivation_of_isProper l hl.1 _ hl.2 with ⟨d⟩; exact ⟨d.cast (by simp)⟩⟩
+
+lemma provable_iff {σ : Sentence L} :
+    Nonempty (T ⊢ σ) ↔ ∃ l, ∃ U : List (Sentence L), (U.map (~·)).subsetSet T ∧ (σ :: U).map Rew.embl ∈ sequents l ∧ isProper l := by
+  exact ⟨by
+    rintro ⟨U, hU, d⟩
+    rcases derivable_iff_isProper.mp (iff_cut.mpr ⟨d⟩) with ⟨l, hl, hmem⟩
+    let l' := (Code.wk ((insert σ U).image Rew.embl).toList, ((σ :: U.toList).map Rew.embl)) :: l
+    have hl' : isProper l' := by simp[isProper, hl]; exact ⟨by simp[List.subset_def], by simp[Finset.insert_eq, hmem]⟩
+    exact ⟨l', U.toList, by
+      simp[List.subsetSet]; intro x hx
+      have : ∃ y ∈ T, ~y = x := by simpa using hU hx
+      rcases this with ⟨y, hy, rfl⟩; simp[hy], by simp, hl'⟩,
+  by rintro ⟨l, U, hU, hl, hproper⟩
+     rcases derivation_of_isProper l hproper _ hl with ⟨d⟩
+     exact ⟨{ 
+       leftHand := U.toFinset
+       hleftHand := by intro x; simp; intro hx; exact ⟨~x, by simp[@hU (~x) (by simp[hx])]⟩
+       derivation := cutWeakeningCut (d.cast (by simp[List.toFinset_map, Finset.insert_eq])) }⟩⟩
+
+end ProofList
+
+end Derivation
+
+
+end FirstOrder
+
+end LO
